generate all VCs for binary search, and prove the easy ones

theories/binary_search_verif.v
@@ -1,5 +1,9 @@
 Require Import VST.floyd.proofauto. (* Import the Verifiable C system *)
+Require Import VST.floyd.sublist.
 Require Import VSTArrayProgs.binary_search. (* Import the AST of this C program *)
+Require Import Lia.
+
+Ltac do_compute_expr_warning::=idtac.
 
 (* The next line is "boilerplate", always required after importing an AST. *)
 Instance CompSpecs : compspecs. make_compspecs prog. Defined.
@@ -11,3 +15,219 @@ match l with
 | _ :: [] => True
 | x :: y :: l' => x <= y /\ sorted l'
 end.
+
+Definition insertion_point (ip : Z) (key : Z) (l : list Z) :=
+0 <= ip <= Zlength l /\
+Forall (fun x => x < key) (sublist 0 ip l) /\
+Forall (fun x => key < x) (sublist ip (Zlength l) l).
+
+Definition binary_search_spec :=
+ DECLARE _binary_search
+  WITH a: val, sh : share, contents : list Z, len : Z, key : Z
+  PRE [ tptr tint, tint, tint ]
+          PROP (readable_share sh;
+                 Zlength contents <= Int.max_signed;
+                 len = Zlength contents;
+                 Int.min_signed <= key <= Int.max_signed;
+                 Forall (fun x => Int.min_signed <= x <= Int.max_signed) contents;
+                 sorted contents)
+          PARAMS (a; Vint (Int.repr len); Vint (Int.repr key))
+          SEP (data_at sh (tarray tint (Zlength contents)) (map Vint (map Int.repr contents)) a)
+  POST [ tint ]
+    EX i:Z,
+         PROP (if in_dec Z.eq_dec key contents then Znth i contents = key else insertion_point (-i - 1) key contents)
+         RETURN (Vint (Int.repr i))
+         SEP (data_at sh (tarray tint (Zlength contents)) (map Vint (map Int.repr contents)) a).
+
+Definition binary_search_while_spec a sh contents len key :=
+EX low : Z, EX high : Z,
+ PROP (0 <= low <= len;
+  Int.min_signed <= high < len;
+  In key contents -> In key (sublist low (high + 1) contents);
+  ~ In key contents -> Forall (fun x => x < key) (sublist 0 low contents) /\ Forall (fun x => key < x) (sublist (high + 1) len contents))
+ LOCAL (temp _a a; temp _low (Vint (Int.repr low)); temp _high (Vint (Int.repr high)); temp _key (Vint (Int.repr key)))
+ SEP (data_at sh (tarray tint (Zlength contents)) (map Vint (map Int.repr contents)) a).
+           
+Definition main_spec :=
+ DECLARE _main
+  WITH gv: globals
+  PRE  [] main_pre prog tt gv
+  POST [ tint ] main_post prog gv.
+
+Definition Gprog : funspecs := ltac:(with_library prog [binary_search_spec; main_spec]).
+
+Lemma sublist_nil1 : forall A i j (l : list A), j <= i -> sublist i j l = [].
+Proof.
+  intros *.
+  apply sublist_nil_gen.
+Qed.
+
+Lemma mean_le : forall i j : Z,
+ i <= j ->
+ i <= i + ((j - i) / 2) <= j.
+Proof.
+intros i j H_ij.
+split.
+- assert (Hle: 0 <= (j - i) / 2) by (apply Zdiv_le_lower_bound; lia).
+  lia.
+- assert (H_ji: 0 <= j - i) by auto with zarith.
+  assert (Hle: (j - i) / 2 <= j - i) by (apply Zdiv_le_upper_bound; lia).
+  lia.
+Qed.
+
+Lemma body_search: semax_body Vprog Gprog f_binary_search binary_search_spec.
+Proof.
+start_function.
+forward.
+forward.
+forward_while (binary_search_while_spec a sh contents len key).
+- entailer!.
+  Exists 0; Exists (Zlength contents - 1).
+  entailer!.
+  split; intros; [|split].
+  * assert (H11 : Zlength contents - 1 + 1 = Zlength contents) by lia.
+    rewrite H11; clear H11.
+    unfold sublist.
+    rewrite skipn_0.
+    rewrite Zlength_correct.
+    assert (Heq: Z.to_nat (Z.of_nat (Datatypes.length contents)) = Datatypes.length contents) by lia.
+    rewrite Heq.
+    rewrite firstn_exact_length.
+    assumption.
+  * unfold sublist.
+    rewrite skipn_0.
+    rewrite firstn_O.
+    apply Forall_nil.
+  * unfold sublist.
+    assert (H11 : Zlength contents - 1 + 1 = Zlength contents) by lia.
+    rewrite H11; clear H11.    
+    rewrite Zlength_correct.
+    assert (Heq: Z.to_nat (Z.of_nat (Datatypes.length contents)) = Datatypes.length contents) by lia.
+    rewrite Heq.
+    rewrite firstn_exact_length.
+    rewrite skipn_exact_length.
+    apply Forall_nil.
+- entailer!.
+- forward.
+  * entailer!.
+    split.
+    + admit.
+    + intro.
+      destruct H0.
+      unfold Int.mone in H11.
+      apply repr_inj_signed in H11; [congruence|idtac|idtac].
+      -- unfold repable_signed.
+         pose proof Int.min_signed_neg as Hneg.
+         set (j := Int.max_signed) in *; compute in j; subst j.
+         lia.
+      -- unfold repable_signed.
+         set (j := Int.min_signed) in *; compute in j; subst j.
+         set (j := Int.max_signed) in *; compute in j; subst j.
+         lia.
+   * assert_PROP (0 <= Int.unsigned (Int.add (Int.repr low) (Int.divs (Int.repr (high - low)) (Int.repr 2))) < Zlength (map Int.repr contents)).
+       entailer!.       
+       admit.
+     assert_PROP ((0 <= Int.unsigned (Int.add (Int.repr low) (Int.divs (Int.repr (high - low)) (Int.repr 2))) < Zlength contents)).
+       entailer!.
+       admit.
+     forward.
+     forward_if.
+     -- forward.
+        ** entailer!.
+           admit.
+        ** entailer!.
+           Exists ((low + ((high - low)/2)) + 1,high).
+           entailer!.
+           admit.
+      -- forward_if.
+         ** forward.
+            ++ entailer!.
+              admit.
+            ++ entailer!.
+              Exists (low,(low + ((high - low)/2)) - 1).
+              entailer!.
+              admit.
+         ** forward.
+            assert (H_key_eq:
+             Int.signed (Int.repr (Znth (Int.unsigned (Int.add (Int.repr low) (Int.divs (Int.repr (high - low)) (Int.repr 2)))) contents)) = key) by lia.
+            Exists (low + ((high - low) / 2)).
+            entailer!.
+            case (in_dec _ _); intro.
+            ++ admit.
+            ++ contradict n.
+              admit.
+- forward.
+  + entailer!.
+    set (j := Int.min_signed) in *; compute in j; subst j.
+    set (j := Int.max_signed) in *; compute in j; subst j.
+    set (j := Int.signed Int.zero) in *; compute in j; subst j.
+    lia.
+  + Exists (-low - 1).
+    entailer!.
+    case (in_dec _ _); intro.
+    * specialize (H6 i).
+      contradict H6.
+      assert (Hlow: high + 1 <= low) by lia.
+      rewrite sublist_nil1; auto.
+    * admit.
+Admitted.
+
+(*
+Lemma sorted_array_index_elt_le : 
+  (forall (intP_a_1_4_alloc_table_at_L:(alloc_table intP)),
+   (forall (intP_intM_a_1_4_at_L:(memory intP int32)),
+    (forall (a_1_0:(pointer intP)),
+     (forall (len_0_0:Z),
+      ((offset_min intP_a_1_4_alloc_table_at_L a_1_0) <= 0 /\
+       (offset_max intP_a_1_4_alloc_table_at_L a_1_0) >= (len_0_0 - 1) ->
+       ((sorted a_1_0 0 (len_0_0 - 1) intP_intM_a_1_4_at_L) ->
+        (forall (i_3:Z),
+         (forall (j_0:Z),
+          (0 <= i_3 /\ i_3 <= (len_0_0 - 1) ->
+           (0 <= j_0 /\ j_0 <= (len_0_0 - 1) ->
+            (i_3 <= j_0 ->
+             (integer_of_int32
+              (select intP_intM_a_1_4_at_L (shift a_1_0 i_3))) <=
+             (integer_of_int32
+              (select intP_intM_a_1_4_at_L (shift a_1_0 j_0)))))))))))))).
+Proof.
+move => alloc_table mem a len [H_min H_max] H_srt i j.
+move: i.
+elim/(well_founded_ind (Zwf_well_founded 0)): j.
+move => x H_ind i H_x H_j H_ix.
+have H_ltx: i = x \/ i < x by omega.
+elim H_ltx => H_ltx'; first by rewrite H_ltx'; auto with zarith.  
+suff H_lt: integer_of_int32 (select mem (shift a (x-1))) <= integer_of_int32 (select mem (shift a x)).
+- suff H_ltm: integer_of_int32 (select mem (shift a i)) <= integer_of_int32 (select mem (shift a (x-1))) by auto with zarith.
+  by apply H_ind; rewrite /Zwf; auto with zarith.
+- pose proof (H_srt (x-1)) as H_ran.
+  move: H_ran.
+  have ->: x - 1 + 1 = x by auto with zarith.
+  move => H_ran.
+  by apply H_ran; auto with zarith.
+Qed.
+
+Lemma sorted_array_index_lt : 
+  (forall (intP_a_2_5_alloc_table_at_L:(alloc_table intP)),
+   (forall (intP_intM_a_2_5_at_L:(memory intP int32)),
+    (forall (a_2:(pointer intP)),
+     (forall (len_1:Z),
+      ((offset_min intP_a_2_5_alloc_table_at_L a_2) <= 0 /\
+       (offset_max intP_a_2_5_alloc_table_at_L a_2) >= (len_1 - 1) ->
+       ((sorted a_2 0 (len_1 - 1) intP_intM_a_2_5_at_L) ->
+        (forall (i_4:Z),
+         (forall (j_1:Z),
+          (0 <= i_4 /\ i_4 <= (len_1 - 1) ->
+           (0 <= j_1 /\ j_1 <= (len_1 - 1) ->
+            ((integer_of_int32 (select intP_intM_a_2_5_at_L (shift a_2 i_4))) <
+             (integer_of_int32 (select intP_intM_a_2_5_at_L (shift a_2 j_1))) ->
+             i_4 < j_1))))))))))).
+Proof.
+move => alloc_table mem a len H_ran H_srt i j H_lei H_lej.
+elim (Z_lt_ge_dec i j) => H_dec; first by [].
+have H_ji: j <= i by auto with zarith.
+have H_le_le: integer_of_int32 (select mem (shift a j)) <= integer_of_int32 (select mem (shift a i)).
+  by apply (sorted_array_index_elt_le _ _ _ _ H_ran H_srt _ _ H_lej H_lei).
+by move => H_lt; auto with zarith.
+Qed.
+*)
